src/program_proof/tulip/program/replica/replica.v
@@ -1,4 +1,5 @@
-From Perennial.program_proof.tulip.invariance Require Import validate execute accept.
+From Perennial.program_proof.tulip.invariance Require Import validate execute accept learn.
+From Perennial.program_proof Require Import std_proof.
 From Perennial.program_proof.tulip.program Require Import prelude.
 From Perennial.program_proof.tulip.program.replica Require Import
   replica_repr replica_accept replica_acquire replica_bump_key replica_finalized
@@ -11,15 +12,18 @@ From Perennial.program_proof.tulip.program.index Require Import index.
 Section replica.
   Context `{!heapGS Σ, !tulip_ghostG Σ}.
 
-  Definition own_replica (rp : loc) (gid rid : u64) γ α : iProp Σ :=
-    ∃ (lsna : u64) (cm : gmap nat bool) (histm : gmap dbkey dbhist)
+  Definition own_replica_histm (rp : loc) (histm : gmap dbkey dbhist) α : iProp Σ :=
+    ([∗ map] k ↦ h ∈ histm, own_phys_hist_half α k h).
+
+  Definition own_replica_with_cloga_no_lsna
+    (rp : loc) (cloga : dblog) (gid rid : u64) γ α : iProp Σ :=
+    ∃ (cm : gmap nat bool) (histm : gmap dbkey dbhist)
       (cpm : gmap nat dbmap) (ptgsm : gmap nat (gset u64))
       (sptsm ptsm : gmap dbkey nat) (psm : gmap nat (nat * bool)) (rkm : gmap nat nat)
-      (clog cloga : dblog) (ilog : list (nat * icommand)),
+      (clog : dblog) (ilog : list (nat * icommand)),
       let log := merge_clog_ilog cloga ilog in
-      "Hlsna"       ∷ rp ↦[Replica :: "lsna"] #lsna ∗
       "Hcm"         ∷ own_replica_cm rp cm ∗
-      "Hphistm"     ∷ ([∗ map] k ↦ h ∈ histm, own_phys_hist_half α k h) ∗
+      "Hhistm"      ∷ own_replica_histm rp histm α ∗
       "Hcpm"        ∷ own_replica_cpm rp cpm ∗
       "Hptsmsptsm"  ∷ own_replica_ptsm_sptsm rp ptsm sptsm ∗
       "Hpsmrkm"     ∷ own_replica_psm_rkm rp psm rkm ∗
@@ -30,18 +34,798 @@ Section replica.
       "#Hclogalb"   ∷ is_txn_log_lb γ gid cloga ∗
       "%Hdompsmrkm" ∷ ⌜dom psm = dom rkm⌝ ∗
       "%Hcloga"     ∷ ⌜prefix clog cloga⌝ ∗
+      "%Hvcpm"      ∷ ⌜map_Forall (λ _ m, valid_wrs m) cpm⌝ ∗
+      "%Hvicmds"    ∷ ⌜Forall (λ nc, (nc.1 <= length cloga)%nat) ilog⌝ ∗
       "%Hexec"      ∷ ⌜execute_cmds log = LocalState cm histm cpm ptgsm sptsm ptsm psm rkm⌝.
 
-  Definition is_replica (rp : loc) : iProp Σ :=
-    ∃ (mu : loc) (txnlog : loc) (idx : loc) (gid rid : u64) γ α,
-      "#HmuP"     ∷ readonly (rp ↦[Replica :: "mu"] #mu) ∗
-      "#Hlock"    ∷ is_lock tulipNS #mu (own_replica rp gid rid γ α) ∗
-      "#HtxnlogP" ∷ readonly (rp ↦[Replica :: "txnlog"] #txnlog) ∗
-      "#Htxnlog"  ∷ is_txnlog txnlog gid γ ∗
-      "#HidxP"    ∷ readonly (rp ↦[Replica :: "idx"] #idx) ∗
-      "#Hidx"     ∷ is_index idx α ∗
-      "%Hgid"     ∷ ⌜gid ∈ gids_all⌝.
+  Definition own_replica (rp : loc) (gid rid : u64) γ α : iProp Σ :=
+    ∃ (cloga : dblog) (lsna : u64),
+      "Hrp"        ∷ own_replica_with_cloga_no_lsna rp cloga gid rid γ α ∗
+      "Hlsna"      ∷ rp ↦[Replica :: "lsna"] #lsna ∗
+      "%Hlencloga" ∷ ⌜length cloga = uint.nat lsna⌝.
 
+  Definition is_replica_txnlog (rp : loc) gid γ : iProp Σ :=
+    ∃ (txnlog : loc),
+      "#HtxnlogP" ∷ readonly (rp ↦[Replica :: "txnlog"] #txnlog) ∗
+      "#Htxnlog"  ∷ is_txnlog txnlog gid γ.
+
+  Definition is_replica_idx (rp : loc) α : iProp Σ :=
+    ∃ (idx : loc),
+      "#HidxP" ∷ readonly (rp ↦[Replica :: "idx"] #idx) ∗
+      "#Hidx"  ∷ is_index idx α.
+
+  Definition is_replica (rp : loc) : iProp Σ :=
+    ∃ (mu : loc) (gid rid : u64) γ α,
+      "#HmuP"    ∷ readonly (rp ↦[Replica :: "mu"] #mu) ∗
+      "#Hlock"   ∷ is_lock tulipNS #mu (own_replica rp gid rid γ α) ∗
+      "#Htxnlog" ∷ is_replica_txnlog rp gid γ ∗
+      "#Hidx"    ∷ is_replica_idx rp α ∗
+      "#Hinv"    ∷ know_tulip_inv γ ∗
+      "%Hgid"    ∷ ⌜gid ∈ gids_all⌝.
+
+  Theorem wp_Replica__multiwrite rp (tsW : u64) pwrsS pwrsL pwrs histm gid γ α :
+    let ts := uint.nat tsW in
+    let histm' := multiwrite ts pwrs histm in
+    valid_pwrs gid pwrs ->
+    dom histm = keys_all ->
+    safe_extension ts pwrs histm ->
+    ([∗ map] k ↦ h ∈ filter_group gid histm', is_repl_hist_lb γ k h) -∗
+    is_replica_idx rp α -∗
+    {{{ own_dbmap_in_slice pwrsS pwrsL pwrs ∗ own_replica_histm rp histm α }}}
+      Replica__multiwrite #rp #tsW (to_val pwrsS)
+    {{{ RET #(); 
+        own_dbmap_in_slice pwrsS pwrsL pwrs ∗ own_replica_histm rp histm' α
+    }}}.
+  Proof.
+    iIntros (ts histm' Hvw Hdomhistm Hlenhistm) "#Hrlbs #Hidx".
+    iIntros (Φ) "!> [[HpwrsS %Hpwrs] Hhistm] HΦ".
+    wp_rec.
+
+    (*@ func (rp *Replica) multiwrite(ts uint64, pwrs []tulip.WriteEntry) {     @*)
+    (*@     for _, ent := range pwrs {                                          @*)
+    (*@         key := ent.Key                                                  @*)
+    (*@         value := ent.Value                                              @*)
+    (*@         tpl := rp.idx.GetTuple(key)                                     @*)
+    (*@         if value.Present {                                              @*)
+    (*@             tpl.AppendVersion(ts, value.Content)                        @*)
+    (*@         } else {                                                        @*)
+    (*@             tpl.KillVersion(ts)                                         @*)
+    (*@         }                                                               @*)
+    (*@     }                                                                   @*)
+    (*@ }                                                                       @*)
+    iDestruct (own_slice_sz with "HpwrsS") as %Hlenpwrs.
+    iDestruct (own_slice_small_acc with "HpwrsS") as "[HpwrsS HpwrsC]".
+    set P := (λ (i : u64),
+      let pwrs' := list_to_map (take (uint.nat i) pwrsL) in
+      own_replica_histm rp (multiwrite ts pwrs' histm) α)%I.
+    wp_apply (wp_forSlice P with "[] [$HpwrsS Hhistm]"); last first; first 1 last.
+    { (* Loop entry. *)
+      subst P. simpl.
+      rewrite uint_nat_W64_0 take_0 list_to_map_nil.
+      by rewrite multiwrite_empty.
+    }
+    { (* Loop body. *)
+      clear Φ.
+      iIntros (i [k v]) "!>".
+      iIntros (Φ) "(Hhistm & %Hbound & %Hi) HΦ".
+      subst P. simpl.
+      iNamed "Hidx".
+      wp_loadField.
+      (* Prove [k] in the domain of [pwrs] and in [keys_all]. *)
+      apply elem_of_list_lookup_2 in Hi as Hpwrsv.
+      rewrite -Hpwrs elem_of_map_to_list in Hpwrsv.
+      apply elem_of_dom_2 in Hpwrsv as Hdompwrs.
+      assert (Hvk : k ∈ keys_all).
+      { clear -Hvw Hdompwrs. set_solver. }
+      wp_apply (wp_Index__GetTuple with "Hidx"); first apply Hvk.
+      iIntros (tpl) "#Htpl".
+      (* Obtain proof that the current key [k] has not been written. *)
+      pose proof (NoDup_fst_map_to_list pwrs) as Hnd.
+      rewrite Hpwrs in Hnd.
+      pose proof (list_lookup_fmap fst pwrsL (uint.nat i)) as Hk.
+      rewrite Hi /= in Hk.
+      pose proof (not_elem_of_take _ _ _ Hnd Hk) as Htake.
+      rewrite -fmap_take in Htake.
+      apply not_elem_of_list_to_map_1 in Htake as Hnone.
+      (* Adjust the goal. *)
+      rewrite uint_nat_word_add_S; last by word.
+      rewrite (take_S_r _ _ _ Hi) list_to_map_snoc; last done.
+      set pwrs' := (list_to_map _) in Hnone *.
+      assert (is_Some (histm !! k)) as [h Hh].
+      { by rewrite -elem_of_dom Hdomhistm. }
+      (* Obtain the length constraint. *)
+      rewrite /safe_extension in Hlenhistm.
+      set histmwr := filter _ _ in Hlenhistm.
+      assert (Hhistmwrk : histmwr !! k = Some h).
+      { by apply map_lookup_filter_Some_2. }
+      specialize (Hlenhistm _ _ Hhistmwrk). simpl in Hlenhistm.
+      (* Obtain the replicated history lb. *)
+      assert (Hh' : histm' !! k = Some (last_extend ts h ++ [v])).
+      { by rewrite (multiwrite_modified Hpwrsv Hh). }
+      iDestruct (big_sepM_lookup _ _ k with "Hrlbs") as "Hrlb".
+      { apply map_lookup_filter_Some_2; first apply Hh'. simpl.
+        clear -Hdompwrs Hvw. set_solver.
+      }
+      (* Take the physical history out. *)
+      iDestruct (big_sepM_delete with "Hhistm") as "[Hh Hhistm]".
+      { rewrite multiwrite_unmodified; [apply Hh | apply Hnone]. }
+      destruct v as [s |]; wp_pures.
+      { (* Case: [@AppendVersion]. *)
+        wp_apply (wp_Tuple__AppendVersion with "Hrlb Htpl Hh").
+        { apply Hlenhistm. }
+        iIntros "Hh".
+        iDestruct (big_sepM_insert_2 with "Hh Hhistm") as "Hhistm".
+        rewrite insert_delete_insert /multiwrite.
+        erewrite insert_merge_l; last first.
+        { by rewrite Hh. }
+        iApply "HΦ".
+        iFrame "∗ #".
+      }
+      { (* Case: [@KillVersion]. *)
+        wp_apply (wp_Tuple__KillVersion with "Hrlb Htpl Hh").
+        { apply Hlenhistm. }
+        iIntros "Hh".
+        iDestruct (big_sepM_insert_2 with "Hh Hhistm") as "Hhistm".
+        rewrite insert_delete_insert /multiwrite.
+        erewrite insert_merge_l; last first.
+        { by rewrite Hh. }
+        iApply "HΦ".
+        iFrame "∗ #".
+      }
+    }
+    iIntros "[Hhistm HpwrsS]". subst P. simpl.
+    iDestruct ("HpwrsC" with "HpwrsS") as "HpwrsS".
+    wp_pures.
+    iApply "HΦ".
+    rewrite -Hlenpwrs firstn_all -Hpwrs list_to_map_to_list.
+    by iFrame.
+  Qed.
+
+  Theorem wp_Replica__terminated rp (tsW : u64) cm :
+    let ts := uint.nat tsW in
+    {{{ own_replica_cm rp cm }}}
+      Replica__terminated #rp #tsW
+    {{{ RET #(bool_decide (ts ∈ dom cm)); own_replica_cm rp cm }}}.
+  Proof.
+    iIntros (ts Φ) "Hcm HΦ".
+    wp_rec.
+
+    (*@ func (rp *Replica) terminated(ts uint64) bool {                         @*)
+    (*@     _, terminated := rp.txntbl[ts]                                      @*)
+    (*@     return terminated                                                   @*)
+    (*@ }                                                                       @*)
+    iNamed "Hcm".
+    wp_loadField.
+    wp_apply (wp_MapGet with "Htxntbl").
+    iIntros (v ok) "[%Hok Htxntbl]".
+    wp_pures.
+    case_bool_decide as Hts.
+    { destruct ok; last first.
+      { exfalso.
+        apply map_get_false in Hok as [Hnone _].
+        apply elem_of_dom in Hts as [b Hb].
+        symmetry in Hcmabs.
+        pose proof (lookup_kmap_eq_None _ _ _ _ _ Hcmabs Hnone) as Hcontra.
+        specialize (Hcontra ts).
+        unshelve epose proof (Hcontra _) as Hcmts; first word.
+        by rewrite Hb in Hcmts.
+      }
+      iApply "HΦ". by iFrame "∗ %".
+    }
+    { destruct ok.
+      { exfalso.
+        apply map_get_true in Hok.
+        apply not_elem_of_dom in Hts.
+        pose proof (lookup_kmap_eq_None _ _ _ _ _ Hcmabs Hts) as Hcontra.
+        specialize (Hcontra tsW).
+        unshelve epose proof (Hcontra _) as Hcmts; first word.
+        by rewrite Hok in Hcmts.
+      }
+      iApply "HΦ". by iFrame "∗ %".
+    }
+  Qed.
+
+  Theorem wp_Replica__release rp pwrsS pwrsL pwrs ptsm sptsm :
+    valid_wrs pwrs ->
+    {{{ own_dbmap_in_slice pwrsS pwrsL pwrs ∗ own_replica_ptsm_sptsm rp ptsm sptsm }}}
+      Replica__release #rp (to_val pwrsS)
+    {{{ RET #(); 
+        own_dbmap_in_slice pwrsS pwrsL pwrs ∗
+        own_replica_ptsm_sptsm rp (release pwrs ptsm) sptsm
+    }}}.
+  Proof.
+    iIntros (Hvw Φ) "[[HpwrsS %Hpwrs] Hrp] HΦ".
+    wp_rec.
+    iDestruct (own_replica_ptsm_sptsm_dom with "Hrp") as %[Hdomptsm Hdomsptsm].
+
+    (*@ func (rp *Replica) release(pwrs []tulip.WriteEntry) {                   @*)
+    (*@     for _, ent := range pwrs {                                          @*)
+    (*@         key := ent.Key                                                  @*)
+    (*@         rp.releaseKey(key)                                              @*)
+    (*@     }                                                                   @*)
+    (*@ }                                                                       @*)
+    iDestruct (own_slice_sz with "HpwrsS") as %Hlenpwrs.
+    iDestruct (own_slice_small_acc with "HpwrsS") as "[HpwrsS HpwrsC]".
+    set P := (λ (i : u64),
+      let pwrs' := list_to_map (take (uint.nat i) pwrsL) in
+      own_replica_ptsm_sptsm rp (release pwrs' ptsm) sptsm)%I.
+    wp_apply (wp_forSlice P with "[] [$HpwrsS Hrp]"); last first; first 1 last.
+    { (* Loop entry. *)
+      subst P. simpl.
+      rewrite uint_nat_W64_0 take_0 list_to_map_nil.
+      by rewrite release_empty.
+    }
+    { (* Loop body. *)
+      clear Φ.
+      iIntros (i [k v]) "!>".
+      iIntros (Φ) "(Hrp & %Hbound & %Hi) HΦ".
+      subst P. simpl.
+      wp_pures.
+      wp_apply (wp_Replica__releaseKey with "Hrp").
+      iIntros "Hrp".
+      iApply "HΦ".
+      (* Obtain proof that the current key [k] has not been written. *)
+      pose proof (NoDup_fst_map_to_list pwrs) as Hnd.
+      rewrite Hpwrs in Hnd.
+      pose proof (list_lookup_fmap fst pwrsL (uint.nat i)) as Hk.
+      rewrite Hi /= in Hk.
+      pose proof (not_elem_of_take _ _ _ Hnd Hk) as Htake.
+      rewrite -fmap_take in Htake.
+      (* Adjust the goal. *)
+      rewrite uint_nat_word_add_S; last by word.
+      rewrite (take_S_r _ _ _ Hi) list_to_map_snoc; last apply Htake.
+      set pwrs' := list_to_map _.
+      rewrite /release setts_insert; last first.
+      { rewrite -Hpwrs in Hi.
+        apply elem_of_list_lookup_2, elem_of_map_to_list, elem_of_dom_2 in Hi.
+        clear -Hvw Hi Hdomptsm. set_solver.
+      }
+      done.
+    }
+    iIntros "[Hrp HpwrsS]".
+    subst P. simpl.
+    rewrite -Hlenpwrs firstn_all -Hpwrs list_to_map_to_list.
+    iDestruct ("HpwrsC" with "HpwrsS") as "HpwrsS".
+    wp_pures.
+    iApply "HΦ".
+    by iFrame.
+  Qed.
+
+  Theorem wp_Replica__applyCommit
+    rp (tsW : u64) pwrsS pwrsL pwrs cloga gid rid γ α :
+    let ts := uint.nat tsW in
+    let cloga' := cloga ++ [CmdCommit ts pwrs] in
+    valid_pwrs gid pwrs ->
+    group_histm_lbs_from_log γ gid cloga' -∗
+    is_txn_log_lb γ gid cloga' -∗
+    is_replica_idx rp α -∗
+    {{{ own_dbmap_in_slice pwrsS pwrsL pwrs ∗
+        own_replica_with_cloga_no_lsna rp cloga gid rid γ α
+    }}}
+      Replica__applyCommit #rp #tsW (to_val pwrsS)
+    {{{ RET #(); 
+        own_dbmap_in_slice pwrsS pwrsL pwrs ∗ 
+        own_replica_with_cloga_no_lsna rp cloga' gid rid γ α
+    }}}.
+  Proof.
+    iIntros (ts cloga' Hvpwrs) "#Hhistmlb #Hlb' #Hidx".
+    iIntros (Φ) "!> [Hpwrs Hrp] HΦ".
+    wp_rec.
+    (* First establish that applying this commit results does not get stuck. *)
+    rewrite /group_histm_lbs_from_log.
+    destruct (apply_cmds cloga') as [cm' histm' |] eqn:Happly'; last done.
+    (* Also establish connection between executing entire log vs. consistent log. *)
+    iNamed "Hrp".
+    unshelve epose proof (execute_cmds_apply_cmds cloga ilog cm histm _) as Happly.
+    { by eauto 10. }
+
+    (*@ func (rp *Replica) applyCommit(ts uint64, pwrs []tulip.WriteEntry) {    @*)
+    (*@     // Query the transaction table. Note that if there's an entry for @ts in @*)
+    (*@     // @txntbl, then transaction @ts can only be committed. That's why we're not @*)
+    (*@     // even reading the value of entry.                                 @*)
+    (*@     committed := rp.terminated(ts)                                      @*)
+    (*@     if committed {                                                      @*)
+    (*@         return                                                          @*)
+    (*@     }                                                                   @*)
+    (*@                                                                         @*)
+    wp_apply (wp_Replica__terminated with "Hcm").
+    iIntros "Hcm".
+    case_bool_decide as Hterm; wp_pures.
+    { iApply "HΦ".
+      apply elem_of_dom in Hterm as [b Hb].
+      iFrame "∗ # %".
+      iPureIntro. simpl.
+      exists ptgsm.
+      split.
+      { by apply prefix_app_r. }
+      rewrite merge_clog_ilog_snoc_clog; last apply Hvicmds.
+      split.
+      { eapply Forall_impl; first apply Hvicmds. simpl.
+        intros nc Hnc.
+        rewrite length_app /=.
+        clear -Hnc. lia.
+      }
+      rewrite /execute_cmds foldl_snoc /= execute_cmds_unfold Hexec /= Hb.
+      destruct b; first done.
+      by rewrite /apply_cmds foldl_snoc /= apply_cmds_unfold /apply_commit Happly Hb in Happly'.
+    }
+    apply not_elem_of_dom in Hterm.
+    rewrite /apply_cmds foldl_snoc /= apply_cmds_unfold Happly /= Hterm in Happly'.
+    case_decide as Hsafeext; last done.
+    symmetry in Happly'. inv Happly'.
+
+    (*@     rp.multiwrite(ts, pwrs)                                             @*)
+    (*@                                                                         @*)
+    wp_apply (wp_Replica__multiwrite with "Hhistmlb Hidx [$Hpwrs $Hhistm]").
+    { apply Hvpwrs. }
+    { by eapply apply_cmds_dom. }
+    { apply Hsafeext. }
+    iIntros "[Hpwrs Hhistm]".
+
+    (*@     rp.txntbl[ts] = true                                                @*)
+    (*@                                                                         @*)
+    iNamed "Hcm".
+    wp_loadField.
+    wp_apply (wp_MapInsert with "Htxntbl"); first done.
+    iIntros "Htxntbl".
+
+    (*@     // With PCR, a replica might receive a commit even if it is not prepared on @*)
+    (*@     // this replica.                                                    @*)
+    (*@     _, prepared := rp.prepm[ts]                                         @*)
+    (*@                                                                         @*)
+    iNamed "Hcpm".
+    wp_loadField.
+    wp_apply (wp_MapGet with "HprepmS").
+    iIntros (prepS prepared) "[%Hprepared HprepmS]".
+    wp_pures.
+
+    (*@     if prepared {                                                       @*)
+    (*@         rp.release(pwrs)                                                @*)
+    (*@         delete(rp.prepm, ts)                                            @*)
+    (*@     }                                                                   @*)
+    (*@ }                                                                       @*)
+    destruct prepared; wp_pures.
+    { wp_apply (wp_Replica__release with "[$Hpwrs $Hptsmsptsm]").
+      { clear -Hvpwrs. set_solver. }
+      iIntros "[Hpwrs Hptsmsptsm]".
+      wp_loadField.
+      wp_apply (wp_MapDelete with "HprepmS").
+      iIntros "HprepmS".
+      wp_pures.
+      iApply "HΦ".
+      apply map_get_true in Hprepared.
+      iDestruct (big_sepM2_delete_l with "Hprepm") as (m) "(%Hm & _ & Hprepm)".
+      { apply Hprepared. }
+      iAssert ([∗ set] t ∈ dom (delete ts cpm), is_replica_validated_ts γ gid rid t)%I
+        as "#Hrpvds'".
+      { rewrite dom_delete_L.
+        iDestruct (big_sepS_delete _ _ ts with "Hrpvds") as "[_ ?]"; last done.
+        symmetry in Hcpmabs.
+        pose proof (lookup_kmap_eq_Some _ _ _ _ _ _ Hcpmabs Hm) as (ts' & Hts' & Hcpmts).
+        assert (ts' = ts) as -> by word.
+        by apply elem_of_dom.
+      }
+      iClear "Hrpvds".
+      iFrame "∗ # %".
+      iPureIntro. simpl.
+      exists (<[ts := true]> cm), (delete ts ptgsm).
+      split.
+      { rewrite 2!kmap_insert. f_equal; [word | done]. }
+      split.
+      { rewrite 2!kmap_delete. f_equal; [word | done]. }
+      split.
+      { by apply prefix_app_r. }
+      { rewrite merge_clog_ilog_snoc_clog; last apply Hvicmds.
+        split.
+        { by apply map_Forall_delete. }
+        split.
+        { eapply Forall_impl; first apply Hvicmds. simpl.
+          intros nc Hnc.
+          rewrite length_app /=.
+          clear -Hnc. lia.
+        }
+        symmetry in Hcpmabs.
+        pose proof (lookup_kmap_eq_Some _ _ _ _ _ _ Hcpmabs Hm) as (ts' & Hts' & Hcpmts).
+        assert (ts' = ts) as -> by word.
+        by rewrite /execute_cmds foldl_snoc /= execute_cmds_unfold Hexec /= Hterm Hcpmts.
+      }
+    }
+    iDestruct (big_sepM2_dom with "Hprepm") as %Hdomprepm.
+    iApply "HΦ".
+    iFrame "∗ # %".
+    iPureIntro. simpl.
+    exists (<[ts := true]> cm), ptgsm.
+    split.
+    { rewrite 2!kmap_insert. f_equal; [word | done]. }
+    split.
+    { by apply prefix_app_r. }
+    { rewrite merge_clog_ilog_snoc_clog; last apply Hvicmds.
+      split.
+      { eapply Forall_impl; first apply Hvicmds. simpl.
+        intros nc Hnc.
+        rewrite length_app /=.
+        clear -Hnc. lia.
+      }
+      apply map_get_false in Hprepared as [Hnone _].
+      rewrite -not_elem_of_dom Hdomprepm not_elem_of_dom in Hnone.
+      symmetry in Hcpmabs.
+      pose proof (lookup_kmap_eq_None _ _ _ _ _  Hcpmabs Hnone) as Hcpmnone.
+      specialize (Hcpmnone ts).
+      unshelve epose proof (Hcpmnone _) as Hcpmts; first word.
+      by rewrite /execute_cmds foldl_snoc /= execute_cmds_unfold Hexec /= Hterm Hcpmts.
+    }
+  Qed.
+
+  Theorem wp_Replica__applyAbort rp (tsW : u64) cloga gid rid γ α :
+    let ts := uint.nat tsW in
+    let cloga' := cloga ++ [CmdAbort ts] in
+    not_stuck (apply_cmds cloga') ->
+    is_txn_log_lb γ gid cloga' -∗
+    {{{ own_replica_with_cloga_no_lsna rp cloga gid rid γ α }}}
+      Replica__applyAbort #rp #tsW
+    {{{ RET #(); own_replica_with_cloga_no_lsna rp cloga' gid rid γ α }}}.
+  Proof.
+    iIntros (ts cloga' Hns) "#Hlb'".
+    iIntros (Φ) "!> Hrp HΦ".
+    wp_rec.
+    (* First establish that applying this commit results does not get stuck. *)
+    destruct (apply_cmds cloga') as [cm' histm' |] eqn:Happly'; last done.
+    (* Also establish connection between executing entire log vs. consistent log. *)
+    iNamed "Hrp".
+    unshelve epose proof (execute_cmds_apply_cmds cloga ilog cm histm _) as Happly.
+    { by eauto 10. }
+
+    (*@ func (rp *Replica) applyAbort(ts uint64) {                              @*)
+    (*@     // Query the transaction table. Note that if there's an entry for @ts in @*)
+    (*@     // @txntbl, then transaction @ts can only be aborted. That's why we're not @*)
+    (*@     // even reading the value of entry.                                 @*)
+    (*@     aborted := rp.terminated(ts)                                        @*)
+    (*@     if aborted {                                                        @*)
+    (*@         return                                                          @*)
+    (*@     }                                                                   @*)
+    (*@                                                                         @*)
+    wp_apply (wp_Replica__terminated with "Hcm").
+    iIntros "Hcm".
+    case_bool_decide as Hterm; wp_pures.
+    { iApply "HΦ".
+      apply elem_of_dom in Hterm as [b Hb].
+      iFrame "∗ # %".
+      iPureIntro. simpl.
+      exists ptgsm.
+      split.
+      { by apply prefix_app_r. }
+      rewrite merge_clog_ilog_snoc_clog; last apply Hvicmds.
+      split.
+      { eapply Forall_impl; first apply Hvicmds. simpl.
+        intros nc Hnc.
+        rewrite length_app /=.
+        clear -Hnc. lia.
+      }
+      rewrite /execute_cmds foldl_snoc /= execute_cmds_unfold Hexec /= Hb.
+      destruct b; last done.
+      by rewrite /apply_cmds foldl_snoc /= apply_cmds_unfold /apply_abort Happly Hb in Happly'.
+    }
+    apply not_elem_of_dom in Hterm.
+    (* rewrite /apply_cmds foldl_snoc /= apply_cmds_unfold Happly /= Hterm in Happly'. *)
+    (* symmetry in Happly'. inv Happly'. *)
+
+    (*@     rp.txntbl[ts] = false                                               @*)
+    (*@                                                                         @*)
+    iNamed "Hcm".
+    wp_loadField.
+    wp_apply (wp_MapInsert with "Htxntbl"); first done.
+    iIntros "Htxntbl".
+
+    (*@     // Tuples lock are held iff @prepm[ts] contains something (and so we should @*)
+    (*@     // release them by calling @abort).                                 @*)
+    (*@     pwrs, prepared := rp.prepm[ts]                                      @*)
+    (*@                                                                         @*)
+    iNamed "Hcpm".
+    wp_loadField.
+    wp_apply (wp_MapGet with "HprepmS").
+    iIntros (prepS prepared) "[%Hprepared HprepmS]".
+    wp_pures.
+
+    (*@     if prepared {                                                       @*)
+    (*@         rp.release(pwrs)                                                @*)
+    (*@         delete(rp.prepm, ts)                                            @*)
+    (*@     }                                                                   @*)
+    (*@ }                                                                       @*)
+    iDestruct (big_sepM2_dom with "Hprepm") as %Hdomprepm.
+    destruct prepared; wp_pures.
+    { apply map_get_true in Hprepared.
+      assert (is_Some (prepm !! tsW)) as [pwrs Hpwrs].
+      { by rewrite -elem_of_dom -Hdomprepm elem_of_dom. }
+      iDestruct (big_sepM2_delete with "Hprepm") as "[Hpwrs Hprepm]".
+      { apply Hprepared. }
+      { apply Hpwrs. }
+      iDestruct "Hpwrs" as (pwrsL) "Hpwrs".
+      wp_apply (wp_Replica__release with "[$Hpwrs $Hptsmsptsm]").
+      { symmetry in Hcpmabs.
+        pose proof (lookup_kmap_eq_Some _ _ _ _ _ _ Hcpmabs Hpwrs) as (ts' & Hts' & Hcpmts).
+        assert (ts' = ts) as -> by word.
+        by specialize (Hvcpm _ _ Hcpmts).
+      }
+      iIntros "[Hpwrs Hptsmsptsm]".
+      wp_loadField.
+      wp_apply (wp_MapDelete with "HprepmS").
+      iIntros "HprepmS".
+      wp_pures.
+      iApply "HΦ".
+      iAssert ([∗ set] t ∈ dom (delete ts cpm), is_replica_validated_ts γ gid rid t)%I
+        as "#Hrpvds'".
+      { rewrite dom_delete_L.
+        iDestruct (big_sepS_delete _ _ ts with "Hrpvds") as "[_ ?]"; last done.
+        symmetry in Hcpmabs.
+        pose proof (lookup_kmap_eq_Some _ _ _ _ _ _ Hcpmabs Hpwrs) as (ts' & Hts' & Hcpmts).
+        assert (ts' = ts) as -> by word.
+        by apply elem_of_dom.
+      }
+      iClear "Hrpvds".
+      iFrame "∗ # %".
+      iPureIntro. simpl.
+      exists (<[ts := false]> cm), (delete ts ptgsm).
+      split.
+      { rewrite 2!kmap_insert. f_equal; [word | done]. }
+      split.
+      { rewrite 2!kmap_delete. f_equal; [word | done]. }
+      split.
+      { by apply prefix_app_r. }
+      { rewrite merge_clog_ilog_snoc_clog; last apply Hvicmds.
+        split.
+        { by apply map_Forall_delete. }
+        split.
+        { eapply Forall_impl; first apply Hvicmds. simpl.
+          intros nc Hnc.
+          rewrite length_app /=.
+          clear -Hnc. lia.
+        }
+        symmetry in Hcpmabs.
+        pose proof (lookup_kmap_eq_Some _ _ _ _ _ _ Hcpmabs Hpwrs) as (ts' & Hts' & Hcpmts).
+        assert (ts' = ts) as -> by word.
+        by rewrite /execute_cmds foldl_snoc /= execute_cmds_unfold Hexec /= Hterm Hcpmts.
+      }
+    }
+    iApply "HΦ".
+    iFrame "∗ # %".
+    iPureIntro. simpl.
+    exists (<[ts := false]> cm), ptgsm.
+    split.
+    { rewrite 2!kmap_insert. f_equal; [word | done]. }
+    split.
+    { by apply prefix_app_r. }
+    { rewrite merge_clog_ilog_snoc_clog; last apply Hvicmds.
+      split.
+      { eapply Forall_impl; first apply Hvicmds. simpl.
+        intros nc Hnc.
+        rewrite length_app /=.
+        clear -Hnc. lia.
+      }
+      apply map_get_false in Hprepared as [Hnone _].
+      rewrite -not_elem_of_dom Hdomprepm not_elem_of_dom in Hnone.
+      symmetry in Hcpmabs.
+      pose proof (lookup_kmap_eq_None _ _ _ _ _  Hcpmabs Hnone) as Hcpmnone.
+      specialize (Hcpmnone ts).
+      unshelve epose proof (Hcpmnone _) as Hcpmts; first word.
+      by rewrite /execute_cmds foldl_snoc /= execute_cmds_unfold Hexec /= Hterm Hcpmts.
+    }
+  Qed.
+
+  Theorem wp_Replica__apply
+    rp cmd pwrsS cloga gid rid γ α :
+    let cloga' := cloga ++ [cmd] in
+    valid_ccommand gid cmd ->
+    group_histm_lbs_from_log γ gid cloga' -∗
+    is_txn_log_lb γ gid cloga' -∗
+    is_replica_idx rp α -∗
+    {{{ own_pwrs_slice pwrsS cmd ∗
+        own_replica_with_cloga_no_lsna rp cloga gid rid γ α
+    }}}
+      Replica__apply #rp (ccommand_to_val pwrsS cmd)
+    {{{ RET #();
+        own_pwrs_slice pwrsS cmd ∗ 
+        own_replica_with_cloga_no_lsna rp cloga' gid rid γ α
+    }}}.
+  Proof.
+    iIntros (cloga' Hvcmd) "#Hsafe #Hlb' #Hidx".
+    iIntros (Φ) "!> [Hpwrs Hrp] HΦ".
+    wp_rec.
+
+    (*@ func (rp *Replica) apply(cmd txnlog.Cmd) {                              @*)
+    (*@     if cmd.Kind == 1 {                                                  @*)
+    (*@         rp.applyCommit(cmd.Timestamp, cmd.PartialWrites)                @*)
+    (*@     } else if cmd.Kind == 2 {                                           @*)
+    (*@         rp.applyAbort(cmd.Timestamp)                                    @*)
+    (*@     }                                                                   @*)
+    (*@ }                                                                       @*)
+    wp_pures.
+    destruct cmd eqn:Hcmd; wp_pures.
+    { (* Case: CmdCommit. *)
+      destruct Hvcmd as [Hvts Hvpwrs].
+      iDestruct "Hpwrs" as (pwrsL) "Hpwrs".
+      wp_apply (wp_Replica__applyCommit with "[Hsafe] [Hlb'] Hidx [$Hpwrs $Hrp]").
+      { apply Hvpwrs. }
+      { rewrite uint_nat_W64_of_nat; first done. rewrite /valid_ts in Hvts. word. }
+      { rewrite uint_nat_W64_of_nat; first done. rewrite /valid_ts in Hvts. word. }
+      iIntros "[Hpwrs Hrp]".
+      wp_pures.
+      iApply "HΦ".
+      rewrite uint_nat_W64_of_nat; last first.
+      { rewrite /valid_ts in Hvts. word. }
+      by iFrame.
+    }
+    { (* Case: CmdAbort. *)
+      simpl in Hvcmd.
+      rewrite /group_histm_lbs_from_log.
+      destruct (apply_cmds cloga') as [cpm histm |] eqn:Happly; last done.
+      wp_apply (wp_Replica__applyAbort with "[Hlb'] Hrp").
+      { rewrite uint_nat_W64_of_nat; first by rewrite Happly. rewrite /valid_ts in Hvcmd. word. }
+      { rewrite uint_nat_W64_of_nat; first done. rewrite /valid_ts in Hvcmd. word. }
+      iIntros "Hrp".
+      wp_pures.
+      iApply "HΦ".
+      rewrite uint_nat_W64_of_nat; last first.
+      { rewrite /valid_ts in Hvcmd. word. }
+      by iFrame.
+    }
+  Qed.
+
+  Theorem wp_Replica__Start rp :
+    is_replica rp -∗
+    {{{ True }}}
+      Replica__Start #rp
+    {{{ RET #(); True }}}.
+  Proof.
+    iIntros "#Hrp" (Φ) "!> _ HΦ".
+    wp_rec.
+
+    (*@ func (rp *Replica) Start() {                                            @*)
+    (*@     rp.mu.Lock()                                                        @*)
+    (*@                                                                         @*)
+    iNamed "Hrp".
+    wp_loadField.
+    wp_apply (wp_Mutex__Lock with "Hlock").
+    iIntros "[Hlocked Hrp]".
+    wp_pures.
+
+    (*@     for {                                                               @*)
+    (*@         // TODO: a more efficient interface would return multiple safe commands @*)
+    (*@         // at once (so as to reduce the frequency of acquiring Paxos mutex). @*)
+    (*@         // Ghost action: Learn a list of new commands.                  @*)
+    (*@         cmd, ok := rp.txnlog.Lookup(rp.lsna)                            @*)
+    (*@                                                                         @*)
+    set P := (λ b : bool, own_replica rp gid rid γ α ∗ locked #mu)%I.
+    wp_apply (wp_forBreak P with "[] [$Hrp $Hlocked]"); last first.
+    { (* Get out of an infinite loop. *)
+      iIntros "Hrp". wp_pures. by iApply "HΦ".
+    }
+    clear Φ. iIntros "!>" (Φ) "[Hrp Hlocked] HΦ".
+    wp_rec.
+    do 2 iNamed "Hrp".
+    wp_loadField.
+
+    (*@         cmd, ok := rp.txnlog.Lookup(lsn)                                @*)
+    (*@                                                                         @*)
+    iNamed "Htxnlog".
+    wp_loadField.
+    wp_apply (wp_TxnLog__Lookup with "Htxnlog").
+    iInv "Hinv" as "> HinvO" "HinvC".
+    iApply ncfupd_mask_intro; first set_solver.
+    iIntros "Hmask".
+    iNamed "HinvO".
+    (* Take the required group invariant. *)
+    iDestruct (big_sepS_elem_of_acc with "Hgroups") as "[Hgroup HgroupsC]"; first apply Hgid.
+    (* Separate out the ownership of the Paxos log from others. *)
+    iDestruct (group_inv_extract_log_expose_cpool with "Hgroup") as (paxos cpool) "[Hpaxos Hgroup]".
+    (* Obtain validity of command input on cpool. *)
+    iDestruct (group_inv_impl_valid_ccommand_cpool with "[Hgroup Hpaxos]") as %Hvcmds.
+    { iNamed "Hgroup". iFrame. }
+    (* Obtain a lower bound before passing it to Paxos. *)
+    iDestruct (txn_log_witness with "Hpaxos") as "#Hlb".
+    iExists paxos. iFrame.
+    iIntros (paxos') "Hpaxos".
+    (* Obtain prefix between the old and new logs. *)
+    iDestruct (txn_log_prefix with "Hpaxos Hlb") as %Hpaxos.
+    destruct Hpaxos as [cmds Hpaxos].
+    (* Obtain inclusion between the command pool and the log. *)
+    iAssert (⌜cpool_subsume_log cpool paxos'⌝)%I as %Hincl.
+    { iNamed "Hgroup".
+      by iDestruct (txn_log_cpool_incl with "Hpaxos Hcpool") as %?.
+    }
+    (* Transfer validity of command input on cpool to log; used when executing @apply. *)
+    pose proof (set_Forall_Forall_subsume _ _ _ Hvcmds Hincl) as Hvc.
+    (* Obtain prefix between the applied log and the new log; needed later. *)
+    iDestruct (txn_log_prefix with "Hpaxos Hclogalb") as %Hloga.
+    (* Obtain a witness of the new log; needed later. *)
+    iDestruct (txn_log_witness with "Hpaxos") as "#Hlbnew".
+    subst paxos'.
+
+    (*@         // Ghost action: Learn a list of new commands.                  @*)
+    (*@                                                                         @*)
+    iMod (group_inv_learn with "Htxnsys Hkeys Hgroup") as "(Htxnsys & Hkeys & Hgroup)".
+    { apply Hincl. }
+    iDestruct (group_inv_merge_log_hide_cpool with "Hpaxos Hgroup") as "Hgroup".
+    (* Put back the group invariant. *)
+    iDestruct ("HgroupsC" with "Hgroup") as "Hgroups".
+    (* Close the entire invariant. *)
+    iMod "Hmask" as "_".
+    iMod ("HinvC" with "[$Htxnsys $Hkeys $Hgroups $Hrgs]") as "_".
+    iIntros "!>" (cmd ok pwrsS) "[HpwrsS  %Hcmd]".
+    wp_pures.
+
+    (*@         if !ok {                                                        @*)
+    (*@             // Sleep for 1 ms.                                          @*)
+    (*@             rp.mu.Unlock()                                              @*)
+    (*@             primitive.Sleep(1 * 1000000)                                @*)
+    (*@             rp.mu.Lock()                                                @*)
+    (*@             continue                                                    @*)
+    (*@         }                                                               @*)
+    (*@                                                                         @*)
+    destruct ok; wp_pures; last first.
+    { (* Have applied all the commands known to be committed. *)
+      wp_loadField.
+      iClear "Hlb Hlbnew".
+      wp_apply (wp_Mutex__Unlock with "[-HΦ $Hlock $Hlocked]"); first by iFrame "∗ # %".
+      wp_apply wp_Sleep.
+      wp_loadField.
+      wp_apply (wp_Mutex__Lock with "Hlock").
+      iIntros "[Hlocked Hrp]".
+      wp_pures.
+      iApply "HΦ".
+      by iFrame.
+    }
+    (* Obtain a witness for the newly applied log. *)
+    iClear "Hlb".
+    (* Prove the newly applied log is a prefix of the new log. *)
+    assert (Hprefix : prefix (cloga ++ [cmd]) (paxos ++ cmds)).
+    { clear -Hloga Hcmd Hlencloga.
+      destruct Hloga as [l Hl].
+      rewrite Hl.
+      apply prefix_app, prefix_singleton.
+      rewrite Hl lookup_app_r in Hcmd; last lia.
+      by rewrite Hlencloga /= Nat.sub_diag in Hcmd.
+    }
+    iDestruct (txn_log_lb_weaken (cloga ++ [cmd]) with "Hlbnew") as "#Hlb"; first apply Hprefix.
+    (* Obtain lbs of replicated history over the new history map. *)
+    iApply fupd_wp.
+    iInv "Hinv" as "> HinvO" "HinvC".
+    (* Take the required group invariant. *)
+    iNamed "HinvO".
+    iDestruct (big_sepS_elem_of_acc with "Hgroups") as "[Hgroup HgroupsC]"; first apply Hgid.
+    iDestruct (group_inv_witness_group_histm_lbs_from_log with "Hlb Hgroup") as "#Hhistmlb".
+    iDestruct ("HgroupsC" with "Hgroup") as "Hgroups".
+    iMod ("HinvC" with "[$Htxnsys $Hkeys $Hgroups $Hrgs]") as "_".
+    iModIntro.
+
+    (*@         rp.apply(cmd)                                                   @*)
+    (*@                                                                         @*)
+    iAssert (own_replica_with_cloga_no_lsna rp cloga gid rid γ α)%I
+      with "[Hcm Hhistm Hcpm Hptsmsptsm Hpsmrkm Hclog Hilog]" as "Hrp".
+    { iFrame "∗ # %". }
+    wp_apply (wp_Replica__apply with "Hhistmlb Hlb Hidx [$HpwrsS $Hrp]").
+    { rewrite Forall_forall in Hvc.
+      apply Hvc.
+      by apply elem_of_list_lookup_2 in Hcmd.
+    }
+    iIntros "[HpwrsS Hrp]".
+
+
+    (*@         rp.lsna = std.SumAssumeNoOverflow(rp.lsna, 1)                   @*)
+    (*@                                                                         @*)
+    wp_loadField.
+    wp_apply wp_SumAssumeNoOverflow.
+    iIntros (Hnoof).
+    wp_storeField.
+
+    (*@     }                                                                   @*)
+    (*@ }                                                                       @*)
+    iApply "HΦ".
+    iFrame.
+    iPureIntro.
+    rewrite uint_nat_word_add_S; last word.
+    rewrite length_app /= Hlencloga.
+    lia.
+  Qed.
 
   Definition finalized_outcome γ ts res : iProp Σ :=
     match res with
@@ -79,7 +863,7 @@ Section replica.
     (*@         }                                                               @*)
     (*@     }                                                                   @*)
     (*@                                                                         @*)
-    iNamed "Hrp". iNamed "Hcm".
+    do 2 iNamed "Hrp". iNamed "Hcm".
     wp_loadField.
     wp_apply (wp_MapGet with "Htxntbl").
     iIntros (cmted bdone) "[%Hcmted Htxntbl]".
@@ -106,9 +890,9 @@ Section replica.
           pose proof (apply_cmds_mono_cm Hprefix Hrsm Happly) as Hcmrp.
           pose proof (lookup_weaken _ _ _ _ Hcmrpts Hcmrp) as Hcmts.
           rewrite Hcm lookup_omap_Some in Hcmts.
-          destruct Hcmts as (st & Hstcmted & Hst).
-          destruct st; [done | | done].
-          by iDestruct (big_sepM_lookup with "Hsafestm") as "Hcmted"; first apply Hst.
+          destruct Hcmts as (status & Hstcmted & Hstatus).
+          destruct status; [done | | done].
+          by iDestruct (big_sepM_lookup with "Hsafestm") as "Hcmted"; first apply Hstatus.
         }
         iMod ("HinvC" with "HinvO") as "_".
         by iFrame "∗ # %".
@@ -133,9 +917,9 @@ Section replica.
           pose proof (apply_cmds_mono_cm Hprefix Hrsm Happly) as Hcmrp.
           pose proof (lookup_weaken _ _ _ _ Hcmrpts Hcmrp) as Hcmts.
           rewrite Hcm lookup_omap_Some in Hcmts.
-          destruct Hcmts as (st & Hstabted & Hst).
-          destruct st; [done | done |].
-          by iDestruct (big_sepM_lookup with "Hsafestm") as "Habted"; first apply Hst.
+          destruct Hcmts as (status & Hstabted & Hstatus).
+          destruct status; [done | done |].
+          by iDestruct (big_sepM_lookup with "Hsafestm") as "Habted"; first apply Hstatus.
         }
         iMod ("HinvC" with "HinvO") as "_".
         by iFrame "∗ # %".
@@ -208,7 +992,7 @@ Section replica.
     (*@         return tulip.REPLICA_OK                                         @*)
     (*@     }                                                                   @*)
     (*@                                                                         @*)
-    iNamed "Hrp". iNamed "Hcpm".
+    do 2 iNamed "Hrp". iNamed "Hcpm".
     iDestruct (big_sepM2_dom with "Hprepm") as %Hdomprepm.
     wp_loadField.
     wp_apply (wp_MapGet with "HprepmS").
@@ -297,6 +1081,7 @@ Section replica.
       iApply (big_sepS_insert_2 ts with "Hvd Hrpvds").
     }
     iClear "Hrpvds".
+    iDestruct (safe_txn_pwrs_impl_valid_wrs with "Hsafepwrs") as %Hvw.
     iFrame "∗ # %".
     iModIntro.
     iPureIntro. simpl.
@@ -305,7 +1090,17 @@ Section replica.
     { rewrite 2!kmap_insert. f_equal; [word | done]. }
     split; first done.
     rewrite merge_clog_ilog_snoc_ilog; last done.
-    by rewrite /execute_cmds foldl_snoc execute_cmds_unfold Hexec /=.
+    split.
+    { by apply map_Forall_insert_2. }
+    split.
+    { rewrite Forall_forall.
+      intros [n c] Hilog. simpl.
+      apply elem_of_app in Hilog as [Hilog | Hnewc].
+      { rewrite Forall_forall in Hvicmds. by specialize (Hvicmds _ Hilog). }
+      rewrite elem_of_list_singleton in Hnewc.
+      by inv Hnewc.
+    }
+    { by rewrite /execute_cmds foldl_snoc execute_cmds_unfold Hexec /=. }
   Qed.
 
   Definition try_accept_outcome γ gid rid ts rank pdec res : iProp Σ :=
@@ -370,7 +1165,7 @@ Section replica.
     (*@         return tulip.REPLICA_STALE_COORDINATOR                          @*)
     (*@     }                                                                   @*)
     (*@                                                                         @*)
-    iNamed "Hrp".
+    do 2 iNamed "Hrp".
     wp_apply (wp_Replica__lowestRank with "Hpsmrkm").
     iIntros (rankl ok) "[Hpsmrkm %Hok]".
     wp_pures.
@@ -408,7 +1203,7 @@ Section replica.
     iMod (replica_inv_accept ts rank dec with "[Hgpsl] Hclog Hilog Hrp")
       as "(Hclog & Hilog & Hrp & #Hacc)".
     { apply Hexec. }
-    { simpl.
+    { rewrite /accept_requirement.
       destruct ok; rewrite Hok; last done.
       apply Classical_Prop.not_and_or in Hcase.
       destruct Hcase as [? | Hge]; first done.
@@ -436,7 +1231,15 @@ Section replica.
     { by rewrite 2!dom_insert_L Hdompsmrkm. }
     split; first done.
     rewrite merge_clog_ilog_snoc_ilog; last done.
-    by rewrite /execute_cmds foldl_snoc execute_cmds_unfold Hexec /=.
+    split.
+    { rewrite Forall_forall.
+      intros [n c] Hilog. simpl.
+      apply elem_of_app in Hilog as [Hilog | Hnewc].
+      { rewrite Forall_forall in Hvicmds. by specialize (Hvicmds _ Hilog). }
+      rewrite elem_of_list_singleton in Hnewc.
+      by inv Hnewc.
+    }
+    { by rewrite /execute_cmds foldl_snoc execute_cmds_unfold Hexec /=. }
   Qed.
 
   Theorem wp_Replica__logFastPrepare (rp : loc) (ts : u64) (pwrs : Slice.t) (ptgs : Slice.t) :
@@ -511,7 +1314,7 @@ Section replica.
     (*@         return tulip.REPLICA_OK                                         @*)
     (*@     }                                                                   @*)
     (*@                                                                         @*)
-    iNamed "Hrp".
+    do 2 iNamed "Hrp".
     wp_apply (wp_Replica__lastProposal with "Hpsmrkm").
     iIntros (rank dec ok) "[Hpsmrkm %Hok]".
     wp_pures.
@@ -593,7 +1396,7 @@ Section replica.
       iMod (replica_inv_accept ts O false with "[] Hclog Hilog Hrp")
         as "(Hclog & Hilog & Hrp & #Hacc)".
       { apply Hexec. }
-      { simpl.
+      { rewrite /accept_requirement.
         destruct (rkm !! ts) as [r |] eqn:Hr; last done.
         apply elem_of_dom_2 in Hr.
         by rewrite -not_elem_of_dom Hdompsmrkm in Hok.
@@ -618,7 +1421,15 @@ Section replica.
       { by rewrite 2!dom_insert_L Hdompsmrkm. }
       split; first done.
       rewrite merge_clog_ilog_snoc_ilog; last done.
-      by rewrite /execute_cmds foldl_snoc execute_cmds_unfold Hexec /=.
+      split.
+      { rewrite Forall_forall.
+        intros [n c] Hilog. simpl.
+        apply elem_of_app in Hilog as [Hilog | Hnewc].
+        { rewrite Forall_forall in Hvicmds. by specialize (Hvicmds _ Hilog). }
+        rewrite elem_of_list_singleton in Hnewc.
+        by inv Hnewc.
+      }
+      { by rewrite /execute_cmds foldl_snoc execute_cmds_unfold Hexec /=. }
     }
     iDestruct "Hptsmsptsm" as "(Hptsmsptsm & %Hvptsm & %Hvsptsm)".
 
@@ -662,7 +1473,7 @@ Section replica.
     { rewrite merge_clog_ilog_snoc_ilog; last done.
       by rewrite /execute_cmds foldl_snoc execute_cmds_unfold Hexec /=.
     }
-    { simpl.
+    { rewrite /accept_requirement.
       destruct (rkm !! ts) as [r |] eqn:Hr; last done.
       apply elem_of_dom_2 in Hr.
       by rewrite -not_elem_of_dom Hdompsmrkm in Hok.
@@ -691,6 +1502,7 @@ Section replica.
       iFrame "Hvd Hacc".
     }
     iClear "Hfpw".
+    iDestruct (safe_txn_pwrs_impl_valid_wrs with "Hsafepwrs") as %Hvw.
     iFrame "∗ # %".
     iPureIntro. simpl.
     exists (<[ts := ∅]> ptgsm).
@@ -701,7 +1513,21 @@ Section replica.
     split; first done.
     do 2 (rewrite merge_clog_ilog_snoc_ilog; last done).
     rewrite /execute_cmds foldl_snoc execute_cmds_unfold.
-    by rewrite /execute_cmds foldl_snoc execute_cmds_unfold Hexec /=.
+    split.
+    { by apply map_Forall_insert_2. }
+    split.
+    { rewrite Forall_forall.
+      intros [n c] Hilog. simpl.
+      apply elem_of_app in Hilog as [Hilog | Hnewc].
+      { apply elem_of_app in Hilog as [Hilog | Hnewc].
+        { rewrite Forall_forall in Hvicmds. by specialize (Hvicmds _ Hilog). }
+        rewrite elem_of_list_singleton in Hnewc.
+        by inv Hnewc.
+      }
+      rewrite elem_of_list_singleton in Hnewc.
+      by inv Hnewc.
+    }
+    { by rewrite /execute_cmds foldl_snoc execute_cmds_unfold Hexec /=. }
   Qed.
 
 End replica.
